atomic_pcas.v
@@ -1,9 +1,8 @@
 From iris.program_logic Require Export weakestpre hoare.
-From iris.heap_lang Require Export lang.
-From iris.heap_lang Require Import proofmode notation.
+From iris.heap_lang Require Export lang proofmode notation.
 From iris.heap_lang.lib Require Import spin_lock.
 From iris.algebra Require Import dec_agree frac.
-From iris_atomic Require Import atomic atomic_sync.
+From iris_atomic Require Import atomic_pcas'.
 Import uPred.
 
 Section atomic_pair.
