simple_sync.v
@@ -3,7 +3,7 @@ From iris.heap_lang Require Export lang.
 From iris.heap_lang Require Import proofmode notation.
 From iris.heap_lang.lib Require Import spin_lock.
 From iris.algebra Require Import dec_agree frac.
-From iris_atomic Require Import atomic atomic_sync.
+From iris_atomic Require Import sync.
 Import uPred.
 
 Definition mk_sync: val :=
