sync.v
@@ -1,0 +1,18 @@
+From iris.program_logic Require Export weakestpre hoare.
+From iris.heap_lang Require Export lang.
+From iris.heap_lang Require Import proofmode notation.
+
+Section sync.
+  Context `{!heapG Σ} (N : namespace).
+  
+  Definition synced R (f' f: val) :=
+    (□ ∀ P Q (x: val), ({{ R ★ P x }} f x {{ v, R ★ Q x v }}) → ({{ P x }} f' x {{ v, Q x v }}))%I.
+
+  Definition is_syncer (R: iProp Σ) (s: val) :=
+    (∀ (f : val), WP s f {{ f', synced R f' f }})%I.
+
+  Definition mk_syncer_spec (mk_syncer: val) :=
+    ∀ (R: iProp Σ) (Φ: val -> iProp Σ),
+      heapN ⊥ N →
+      heap_ctx ★ R ★ (∀ s, □ (is_syncer R s) -★ Φ s) ⊢ WP mk_syncer #() {{ Φ }}.
+End sync.
